reify/reify_triple.v
@@ -7,6 +7,9 @@ Require Import types.
 Require Import reify_derives.
 Require Import functions.
 Require Import MirrorShard.ReifyExpr MirrorShard.ReifySepExpr.
+Require Import msl.Axioms.
+Require Import MirrorShard.Env.
+Require Import c_to_expr.
 
 Local Open Scope logic.
 
@@ -22,24 +25,26 @@ Record Triple := mkTriple
   Tlocal : list expr;
   Tsep : list sepE;
   Tcommand : statement;
-  Tpost : ret_assert
+  Tpost : ret_assert(*;
+  Tret : option exitkind*)
 }.
 
 Section denotation.
 
-Variable functions : functions our_types.
-Variable preds : Sep.predicates our_types.
-Variable uvars : Expr.env our_types.
+Variable functions : functions (all_types_r (@nil type)).
+Variable preds : Sep.predicates (all_types_r (@nil type)).
+Variable uvars : Expr.env (all_types_r (@nil type)).
 
 
 Definition reflect_prop e := force_Opt (exprD functions uvars nil e tvProp) False.
 Definition False' (_ : environ) := False.
+Definition True' (_ : environ) := True.
 Definition reflect_local (e: expr) :=  (force_Opt (exprD functions uvars nil e (Expr.tvType 17)) False').
 
 Definition s_reflect (e : sepE) := 
 match e with
 | all_lift sexpr => `(Sep.sexprD functions preds uvars nil sexpr)
-| one_arg expr => force_Opt (exprD functions uvars nil expr (Expr.tvType 18)) FF
+| one_arg expr => force_Opt (exprD functions uvars nil expr (Expr.tvType 18)) TT
 end.
 
 (*Redefining map so we won't unfold user maps when we reflect *)
@@ -70,13 +75,13 @@ Definition TripleD t :=
 End denotation.
                 
 (*shouldn't need these, can probably do this as part of reification*)
-Ltac change_eqs' l :=
+(*Ltac change_eqs' l :=
 try
 match l with
 | ?H :: ?T => match H with
                 | `(eq ?l) (eval_id ?r) => change H with (functions.lift_eq l r)
               end; change_eqs' T
-end.
+end.*)
 
 Ltac change_eqs :=
 match goal with 
@@ -210,174 +215,61 @@ try abbreviate_triple.
 
 Import ListNotations.
 
-Fixpoint ident_to_expr (i: ident) :=
-match i with 
-  | xI p' => Func functions.xIp_f [ident_to_expr p']
-  | xO p' => Func functions.xOp_f [ident_to_expr p']
-  | xH => Func functions.xHp_f []
-end. 
-
-Fixpoint pos_to_expr (p: positive) :=
-match p with
-  | xI p' => Func functions.xI_f [pos_to_expr p']
-  | xO p' => Func functions.xO_f [pos_to_expr p']
-  | xH => Func functions.xH_f []
-end.
-
-Definition Z_to_expr (z : Z) :=
-match z with
-| Zpos p => Func functions.Zpos_f [pos_to_expr p]
-| Zneg p => Func functions.Zneg_f [pos_to_expr p]
-| Z0 => Func functions.Z0_f []
-end.
-
-Definition int32_to_expr (i : int) :=
-Func int_repr_f [Z_to_expr (Int.intval i)].
-
-Definition int64_to_expr (i : int64) :=
-Func int_repr_f [Z_to_expr (Int64.intval i)].
-
-Definition optN_to_expr (on : option N) :=
-match on with
-    Some N0 => Func Some_N_f [Func N0_f []]
-  | Some (Npos p) => Func Some_N_f [Func Npos_f [pos_to_expr p]]
-  | None => Func None_N_f []
-end.
-
-Definition bool_to_expr (b: bool) :=
-match b with
-| true => Func true_f []
-| false => Func false_f []
-end.
-
-Definition attr_to_expr (a : attr) :=
-match a with
-{| attr_volatile := b; attr_alignas := a |} =>
-Func mk_attr_f [bool_to_expr b; optN_to_expr a]
-end.
-
-Definition intsize_to_expr (sz : intsize) :=
-match sz with
-I8 => Func I8_f []
-| I16 => Func I16_f []
-| I32 => Func I32_f [] 
-| IBool => Func IBool_f []
-end.
-
-Definition floatsize_to_expr (sz: floatsize) :=
-match sz with
-F32 => Func F32_f []
-| F64 => Func F64_f []
-end.
-
-
-Definition signedness_to_expr (s: signedness) :=
-match s with
-  Signed => Func signed_f [] 
-| Unsigned => Func unsigned_f []
-end.
-
-
-Fixpoint type_to_expr (ty : Ctypes.type) :=
-match ty with
-  | Tvoid => Func functions.Tvoid_f []
-  | Tint sz sn attr => Func functions.Tint_f [intsize_to_expr sz; signedness_to_expr sn; attr_to_expr attr]
-  | Tlong sg attr => Func functions.Tlong_f [signedness_to_expr sg; attr_to_expr attr]
-  | Tfloat fs attr => Func functions.Tfloat_f [floatsize_to_expr fs; attr_to_expr attr] 
-  | Tpointer t attr => Func functions.Tpointer_f [type_to_expr t; attr_to_expr attr] 
-  | Tarray t z attr => Func functions.Tpointer_f [type_to_expr t; Z_to_expr z; attr_to_expr attr] 
-  | Tfunction tl t => Func functions.Tfunction_f [typelist_to_expr tl; type_to_expr t]
-  | Tstruct id fl attr => Func Tstruct_f [ident_to_expr id; fieldlist_to_expr fl; attr_to_expr attr]
-  | Tunion id fl attr => Func Tunion_f [ident_to_expr id; fieldlist_to_expr fl; attr_to_expr attr]
-  | Tcomp_ptr id attr => Func Tcomp_ptr_f [ident_to_expr id; attr_to_expr attr]
-end
-
-with typelist_to_expr tl :=
-match tl with
-  Ctypes.Tnil => Func Tnil_f []
-| Ctypes.Tcons h t => Func Tcons_f [type_to_expr h; typelist_to_expr t]
-end
-
-with fieldlist_to_expr fl :=
-match fl with 
- Fnil => Func Fnil_f []
-| Fcons id ty t => Func Fcons_f [ident_to_expr id; type_to_expr ty; fieldlist_to_expr t]
-end.
-
-Definition unop_to_expr o :=
-match o with
-    Onotbool => Func Onotbool_f []
-  | Onotint => Func Onotint_f []
-  | Oneg => Func Oneg_f []
-end.
-
-Print Cop.binary_operation.
-Definition binop_to_expr o :=
-match o with
-    Oadd => Func Oadd_f []
-  | Osub => Func Osub_f []
-  | Omul => Func Omul_f []
-  | Odiv => Func Odiv_f []
-  | Omod => Func Omod_f []
-  | Oand => Func Oand_f []
-  | Oor => Func Oor_f [] 
-  | Oxor => Func Oxor_f []
-  | Oshl => Func Oshl_f []
-  | Oshr => Func Oshr_f []
-  | Oeq => Func Oeq_f [] 
-  | One => Func One_f [] 
-  | Olt => Func Olt_f [] 
-  | Ogt => Func Ogt_f []
-  | Ole => Func Ole_f [] 
-  | Oge => Func Oge_f []
-end.
-
-Definition float_to_expr (f:float) := Func functions.O_f []. (*Placeholder, deal with floats later*)
 
 Fixpoint msubst_eval_expr (P: PTree.t expr) (e: Clight.expr) 
- : expr :=
+ : option expr :=
  match e with
- | Econst_int i ty => Func functions.vint_f [int32_to_expr i]
- | Econst_long i ty => Func functions.vlong_f [int64_to_expr i]
- | Econst_float f ty => Func functions.vfloat_f [float_to_expr f]
- | Etempvar id ty => match P ! id with
-                                 | Some v => v
-                                 | None => Func (functions.eval_id_f nil) [ident_to_expr id] (*eval_id_lift?? maybe fail... this isn't right though, fail might be right, this may not be possible*) 
-                                 end
+ | Econst_int i ty => Some (Func functions.vint_f [int32_to_expr i])
+ | Econst_long i ty => Some (Func functions.vlong_f [int64_to_expr i])
+ | Econst_float f ty => None (*Some (Func functions.vfloat_f [float_to_expr f])*)
+ | Etempvar id ty => P ! id
  | Eaddrof a ty => msubst_eval_lvalue_expr P a 
- | Eunop op a ty =>  Func eval_unop_f [unop_to_expr op; type_to_expr ty; 
-                                       msubst_eval_expr P a  ]
- | Ebinop op a1 a2 ty => Func eval_binop_f [binop_to_expr op; type_to_expr ty;
-                                            msubst_eval_expr P a1  ;
-                                            msubst_eval_expr P a2  ]
- | Ecast a ty => Func eval_cast_f [type_to_expr (Clight.typeof a); type_to_expr ty;
-                                   msubst_eval_expr P a  ]
- | Evar id ty => (*Func deref_noload [type_to_expr ty; ]*) Func functions.O_f [] (*shouldn't happen?*)
- | Ederef a ty => Func deref_noload_f [type_to_expr ty; 
-                                       Func force_ptr_f 
-                                            [msubst_eval_expr P a ]]
- | Efield a i ty => Func deref_noload_f [type_to_expr ty;
-                                          Func eval_field_f
-                                               [type_to_expr (Clight.typeof a);
-                                                 ident_to_expr i;
-                                                 msubst_eval_expr P a ]]
+ | Eunop op a _ => option_map (fun v => Func eval_unop_f [unop_to_expr op; type_to_expr (Clight.typeof a); v]) (msubst_eval_expr P a)  
+ | Ebinop op a1 a2 ty => 
+   match (msubst_eval_expr P a1), (msubst_eval_expr P a2) with
+     | Some v1, Some v2 => 
+       Some (Func eval_binop_f [binop_to_expr op; type_to_expr (Clight.typeof a1);
+                          type_to_expr (Clight.typeof a2);
+                          v1 ; v2 ])
+     | _, _ => None
+   end
+ | Ecast a ty => option_map (fun v => 
+                               Func eval_cast_f [type_to_expr (Clight.typeof a); type_to_expr ty;
+                                                 v ])
+                            (msubst_eval_expr P a )
+ | Evar id ty => None
+ | Ederef a ty => 
+   option_map (fun v => (Func deref_noload_f [type_to_expr ty; Func force_ptr_f [v ]]))
+              (msubst_eval_expr P a)
+ | Efield a i ty => 
+   option_map (fun v =>
+   Func deref_noload_f [type_to_expr ty;
+                         Func eval_field_f
+                              [type_to_expr (Clight.typeof a);
+                                ident_to_expr i; v]])
+              (msubst_eval_lvalue_expr P a)
+                                
 end
 with msubst_eval_lvalue_expr (P: PTree.t expr) (e: Clight.expr) := 
        match e with 
-         | Evar id ty => Func functions.O_f []
-         | Ederef a ty => Func force_ptr_f 
-                               [msubst_eval_expr P a ]
-         | Efield a i ty =>  Func eval_field_f
+         | Evar id ty => None
+         | Ederef a ty => 
+           option_map (fun v => Func force_ptr_f 
+                               [v]) (msubst_eval_expr P a)
+         | Efield a i ty =>  
+           option_map (fun v =>  Func eval_field_f
                                   [type_to_expr (Clight.typeof a);
-                                    ident_to_expr i;
-                                    msubst_eval_lvalue_expr P a ]
-         | _  =>  Func functions.O_f []
+                                    ident_to_expr i; v ])
+                                  (msubst_eval_lvalue_expr P a)
+         | _  =>  None
  end.
 
 
 
 (*Compute lift_eq_f.*)
-(*111%nat is supposed to be Compute lift_eq_f. lift_eq_f breaks things for some reason*)
+(*114%nat is supposed to be Compute lift_eq_f. lift_eq_f breaks things for some reason*)
+Definition reflect_id (funcs' : functions (all_types_r (@nil type))) uvars e := force_Opt (exprD funcs' uvars nil e ident_tv) 1%positive.
+(*
 Definition reflect_id (id_e: expr) (funcs:  list (signature (all_types_r []))) : positive := 
 match id_e with
   | Func id [] => 
@@ -388,33 +280,35 @@ match id_e with
       | _ => 1%positive
     end
   | _ => 1%positive
-end. 
-Check PTree.set.
+end. *)
 
-Fixpoint make_P' P l funcs :=
+Fixpoint make_P' P l funcs' uenv:=
 match l with
-Func 111%nat [val_e; id_e] :: t => make_P' (PTree.set (reflect_id id_e funcs) val_e P) t funcs
+Func 114%nat [val_e; id_e] :: t => make_P' (PTree.set (reflect_id funcs' uenv id_e) val_e P) t funcs' uenv
 | _ => P
 end.
 
-Definition make_P funcs l :=
-make_P' (PTree.empty expr) l funcs.
-Check lift_eq.
+Definition make_P funcs uenv l :=
+make_P' (PTree.empty expr) l funcs uenv.
 
-Definition symexe (t : Triple) funcs : Triple :=
+Definition symexe (t : Triple) funcs uenv : Triple :=
 match (Tcommand t) with
 | (Ssequence (Sset id e) c) => 
- {|Tdelta := Tdelta t; 
-   Tprop := Tprop t;
-   Tlocal := (Func 114%nat [msubst_eval_expr (make_P funcs (Tlocal t)) e; ident_to_expr id] :: Tlocal t);
-   Tsep := Tsep t;
-   Tcommand := c;
-   Tpost := Tpost t
- |}
+  match (msubst_eval_expr (make_P funcs uenv (Tlocal t)) e) with
+    | Some v => 
+      {|Tdelta := update_tycon (Tdelta t) (Sset id e); 
+        Tprop := Tprop t;
+        Tlocal := (Func 114%nat [v ; ident_to_expr id] :: Tlocal t);
+        Tsep := Tsep t;
+        Tcommand := c;
+        Tpost := Tpost t
+      |}
+    | _ => t
+  end
 | _ => t
 end.
 
-Axiom symexe_sound : forall funcs preds uenv trip, TripleD funcs preds uenv (symexe trip funcs) ->
+Axiom symexe_sound : forall funcs preds uenv trip, TripleD funcs preds uenv (symexe trip funcs uenv) ->
 TripleD funcs preds uenv trip.
 
 Ltac reflect_triple :=
@@ -520,6 +414,293 @@ PTree.get PTree.set map Clight.typeof tint tptr tlong tvoid noattr
 
 _w].
 
+
+Ltac simpl_reflect := cbv [Tdelta Tprop Tlocal Tsep PreD Tcommand Tpost] in *.
+
+Ltac simpl_nth H :=
+try match goal with
+[ H : context[nth_error ?f ?n] |- _] => simpl (nth_error f n) in H
+end.
+
+Ltac simpl_reflect_local_H H:=
+repeat (cbv [reflect_local TripleD reflect_Tlocal map'] in H; simpl_reflect; simpl_nth H).
+
+Tactic Notation "simpl_reflect_local" "in" constr(H) := simpl_reflect_local_H H.
+Check exprD.
+
+Definition funcs funcs' := (our_functions nil) ++ funcs'.
+
+
+Definition denote_local_ptree (P: PTree.t expr) funcs' uenv rho:=
+  forall i v val , 
+    Some val = exprD (funcs funcs') uenv nil v val_tv ->
+    PTree.get i P = Some v -> eval_id i rho = val.
+
+Ltac do_n n t :=
+let nn := eval vm_compute in n in
+match nn with
+S ?n' => t; do_n n' t
+| _ => idtac
+end.
+
+Hint Rewrite PTree.gempty : pt.
+Ltac pts := autorewrite with pt in *; try congruence.
+
+Fixpoint id_in_local i l funcs uenv:=
+match l with
+h :: t => match h with
+            | Func 114%nat args => match args with
+                                     | _ :: i2 :: _ => 
+                                       orb (Pos.eqb (reflect_id funcs uenv i2) i) 
+                                           (id_in_local i t funcs uenv)
+                                     | _ => false
+                                    end
+            | _ => false
+          end
+| _ => true
+end.
+Check exprD.
+Inductive locals_wf (funcs' : list (signature (all_types_r []))) uenv : list expr -> Prop :=
+  | locals_wf_nil : locals_wf  funcs' uenv []
+  | locals_wf_cons : forall tl id val v,
+       id_in_local (reflect_id (funcs') uenv id) tl (funcs') uenv = false ->
+       exprD funcs' uenv nil val val_tv = Some v -> 
+       locals_wf funcs' uenv tl ->
+       locals_wf funcs' uenv ((Func (lift_eq_f nil)  [val; id]) :: tl).
+
+Lemma make_P_help : forall locals id id2 funcs' uenv val P 
+(LWF : locals_wf (funcs funcs') uenv locals),
+id_in_local id locals (funcs funcs') uenv = false ->
+(make_P' (PTree.set id val P) locals (funcs funcs') uenv) ! id2 =
+(PTree.set id val (make_P' P locals (funcs funcs') uenv)) ! id2 .
+Proof.
+induction locals; intros. simpl in *. auto.
+inv LWF.
+simpl in *. rewrite orb_false_iff in H. destruct H.
+erewrite IHlocals; eauto.
+repeat rewrite (PTree.gsspec).
+destruct (peq id2 id), (peq id2 (reflect_id (funcs funcs') uenv id0)); subst;
+try congruence.
+subst. rewrite Pos.eqb_refl in *; congruence.
+erewrite IHlocals; eauto. rewrite PTree.gss; auto.
+erewrite IHlocals; eauto. rewrite PTree.gss; auto.
+repeat (erewrite IHlocals; eauto).
+repeat rewrite PTree.gso; auto.
+Qed.
+
+Definition make_P_sound : forall funcs' uenv locals rho 
+(LWF :locals_wf (funcs funcs') uenv locals),
+(fold_right (`and) (`True) (reflect_Tlocal (funcs funcs') uenv locals)) rho->
+denote_local_ptree (make_P (funcs funcs') uenv locals) funcs' uenv rho.
+Proof.
+intros.
+unfold denote_local_ptree; intros.
+simpl in *.
+induction locals; simpl in *. 
+  + unfold make_P in H1. simpl in H1.
+    pts.
+  + inv LWF. unfold make_P in H1. simpl in H1.
+    rewrite make_P_help in *; auto. super_unfold_lift.
+    destruct H. rewrite PTree.gsspec in *.
+    destruct (peq i (reflect_id (funcs funcs') uenv id)); subst.
+      - inv H1. 
+        unfold reflect_local in H.
+        simpl in H.
+        rewrite <- H0 in H. 
+        unfold reflect_id.
+        case_eq (exprD (funcs funcs') uenv [] id ident_tv); intros; try rewrite H1 in *.
+        simpl in H. unfold lift_eq in H. super_unfold_lift. subst.
+        simpl. auto. simpl.
+        inv H.
+      - eapply IHlocals; eauto.
+Qed.
+
+Ltac transl_H H :=
+autorewrite with translate in H. 
+
+Ltac ind1 hyp hyp2 :=
+repeat
+(simpl in *; try congruence; 
+match goal with
+| [ H0 : Some _ = Some _ |- _] => inv H0; try reflexivity; try congruence
+| [ H0 : context[option_map _ (?f ?P ?e)] |- _ ]  =>
+    let c := fresh "Case" in
+    let v := fresh "val" in
+    case_eq (f P e); [intros v c | intros c]; try rewrite c in *
+| [ H0 : context[match (?f ?P ?e) with _ => _ end] |- _] =>
+    let c := fresh "Case" in
+    let v := fresh "val" in
+    case_eq (f P e); [intros v c | intros c]; try rewrite c in *
+| [ H : context[match exprD ?F ?U [] ?v val_tv with _ => _ end ] |- _] => 
+  let c := fresh "Case" in
+  let v := fresh "val" in
+  case_eq (exprD F U [] v val_tv);  [intros v c | intros c]; rewrite c in *
+| [ H : ?F ?P ?e = Some _, 
+    H1 : exprD ?f ?uenv [] ?v val_tv = Some _ |- _] =>
+      solve [super_unfold_lift; simpl; first [erewrite <- hyp2 | repeat erewrite <- hyp]; eauto; reflexivity]
+| [ H0 : context[match exprD (?Funcs) ?uenv [] _ _ with _ => _ end] |- _] => transl_H H0
+
+end).
+
+Lemma msubst_eval_expr_eq:
+  forall P e rho val funcs' uenv val_e, 
+    denote_local_ptree P funcs' uenv rho ->
+    Some val_e = msubst_eval_expr P e ->
+    Some val = exprD (funcs funcs') uenv nil val_e val_tv ->
+    val = eval_expr e rho
+with msubst_eval_lvalue_eq: 
+  forall P e rho val funcs' uenv val_e,
+    denote_local_ptree P funcs' uenv rho ->
+    Some val_e = msubst_eval_lvalue_expr P e ->
+    Some val = exprD (funcs funcs') uenv nil val_e val_tv ->
+    val = eval_lvalue e rho.
+Proof with ind1 msubst_eval_expr_eq msubst_eval_lvalue_eq.
+- intros.
+  destruct e...
+    + simpl in *. case_eq (P ! i); [intros e ce | intros ce]; rewrite ce in *.
+      unfold denote_local_ptree in H.
+      eapply H in H1. simpl. symmetry. apply H1. 
+      congruence.
+      congruence.
+    + simpl. erewrite <- msubst_eval_lvalue_eq; eauto.
+- intros.
+  destruct e...
+Qed.
+
+Lemma wf_locals_P : forall local funcs' uenv id v,
+locals_wf (funcs funcs') uenv local ->
+(make_P (funcs funcs') uenv local) ! id = Some v ->
+exists r, exprD (funcs funcs') uenv [] v val_tv = Some r.
+Proof.
+induction local; intros.
+  unfold make_P in H0. simpl in H0. rewrite PTree.gempty in H0. congruence.
+  simpl in *. inv H. unfold make_P in H0. simpl in H0. rewrite make_P_help in H0; auto.
+  rewrite PTree.gsspec in H0. if_tac in H0. subst. inv H0. rewrite H4; eauto.
+  simpl in *. eapply IHlocal; eauto. 
+Qed.
+
+
+Lemma wf_locals_reflect : forall e funcs' uenv local v,
+locals_wf (funcs funcs') uenv local -> 
+Some v = msubst_eval_expr (make_P (funcs funcs') uenv local) e ->
+exists r, 
+exprD (funcs funcs') uenv [] v val_tv = Some r
+with wf_locals_lvalue_reflect :
+forall e funcs' uenv local v,
+locals_wf (funcs funcs') uenv local -> 
+Some v = msubst_eval_lvalue_expr (make_P (funcs funcs') uenv local) e ->
+exists r, 
+exprD (funcs funcs') uenv [] v val_tv = Some r.
+Proof.
+- destruct e; intros; try solve [inv H0; repeat simpl in *; transl; eauto].
+  + simpl in *. 
+    symmetry in H0. apply wf_locals_P in H0; auto.
+  + simpl in *. 
+    case_eq ((msubst_eval_expr (make_P (funcs funcs') uenv local) e)); intros; rewrite H1 in *;
+    simpl in *; try congruence.
+    inv H0. simpl. transl. 
+    case_eq (exprD (funcs funcs') uenv [] e0 val_tv); intros. eauto.
+    symmetry in H1. eapply wf_locals_reflect in H1. destruct H1. congruence. auto.
+  + simpl in *. case_eq ((msubst_eval_expr (make_P (funcs funcs') uenv local) e)); intros;
+                try rewrite H1 in *; simpl in *; try congruence. inv H0. 
+    simpl. transl. edestruct wf_locals_reflect; eauto. rewrite H0; eauto.
+  + simpl in *. ind1 idtac idtac. simpl; transl.
+    edestruct wf_locals_reflect. eauto. symmetry in Case. apply Case.
+    edestruct wf_locals_reflect. eauto. symmetry in Case0. apply Case0.
+    rewrite H1. rewrite H0. eauto.
+  + ind1 idtac idtac. simpl in *. transl. edestruct wf_locals_reflect; eauto.
+    rewrite H0. eauto.
+  + ind1 idtac idtac. simpl; transl. edestruct wf_locals_lvalue_reflect; eauto.
+    rewrite H0; eauto.
+- destruct e; intros; try solve [inv H0; repeat simpl in *; transl; eauto].
+  + ind1 idtac idtac. simpl in *. edestruct wf_locals_reflect; eauto.
+    rewrite H0; eauto.
+  + ind1 idtac idtac. simpl in *. transl.
+    edestruct (wf_locals_lvalue_reflect); eauto. rewrite H0; eauto.
+Qed.
+ 
+Theorem symexe_sound_s : forall funcs' preds uenv trip
+(LWF : locals_wf (funcs funcs') uenv (Tlocal trip)),
+TripleD (funcs funcs') preds uenv (symexe trip (funcs funcs') uenv) ->
+TripleD (funcs funcs') preds uenv trip.
+intros.
+unfold TripleD.
+destruct trip.
+destruct Tcommand0;
+try solve [unfold symexe in *; simpl in *; auto].
+destruct Tcommand0_1;
+try solve [unfold symexe in *; simpl in *; auto].
+simpl_reflect. unfold symexe in H. simpl_reflect.
+unfold TripleD, PreD, Tlocal, reflect_Tlocal, reflect_Tprop in H.
+revert H. case_eq (msubst_eval_expr (make_P (funcs funcs') uenv Tlocal0) e); intros. simpl in *.
+unfold reflect_local in H0. simpl in H0. edestruct wf_locals_reflect; eauto.
+rewrite H1 in H0. transl_H H0. simpl in H0.
+eapply semax_seq.
+apply sequential'. 
+eapply semax_post; [ | apply forward_setx; auto]. 
+intros.
+Focus 3.
+simpl. 
+ apply H0. intro rho. normalize.
+apply normal_ret_assert_derives.
+entailer!.
+SearchAbout subst.
+Check semax_seq. intros. destruct ek; simpl. 
+
+intros. 
+Check forward_setx.
+Print normal_ret_assert.
+rewrite overridePost_normal'.
+SearchAbout overridePost.
+Check normal_ret_assert.
+intros.  entailer!.
+intro rho. normalize.
+SearchAbout normal_ret_assert.
+apply derives_extract_prop.
+
+ simpl in H.
+symmetry in H0.
+extensionality.
+eapply msubst_eval_expr_eq in H0; eauto.
+Focus 2.
+forward. Focus 2. simpl.
+simpl_reflect_local in H.
+simpl ((force_Opt
+                 (exprD funcs uenv []
+                    (Func 114%nat
+                       [msubst_eval_expr (make_P funcs Tlocal0) e;
+                       ident_to_expr i]) (tvType 17)) False')) in H.
+unfold TripleD in H; unfold PreD in H; simpl in H.
+simpl_reflect_local in H.  simpl in H.
+
+simpl (nth_error funcs 114) in H.
+
+compute (nth_error_funcs 114).
+
+unfold TripleD in H0. simpl_reflect.
+unfold reflect_Tlocal in H0. unfold map' in H0. simpl in H0.
+
+let f := eval vm_compute in funcs in id_this f.
+
+Ltac nth_unfold H :=
+match goal with
+[ H : context[nth_error ?funcs ?id]] 
+
+
+
+
+unfold reflect_local in H0.
+
+Ltac compute_exprD_h H :=
+match goal with
+
+
+ simpl in H0. rewrite H in H0.
+simpl in H0.
+Print closed_wrt_vars. 
+
+*)
+
 Lemma triple : forall p contents sh,
 exists POSTCONDITION,
 semax Delta2
@@ -530,7 +711,6 @@ semax Delta2
 intros. 
 eexists.
 pose_env.
-forward.
 reify_triple.
 apply symexe_sound.
 reflect_triple. simpl. 
